examples/demo/sauto/itrev.v
@@ -1,0 +1,158 @@
+(* Tail-recursive reverse *)
+
+From Hammer Require Import Tactics.
+
+Require List.
+Import List.ListNotations.
+Open Scope list_scope.
+
+Fixpoint itrev {A} (l acc : list A) :=
+  match l with
+  | [] => acc
+  | h :: t => itrev t (h :: acc)
+  end.
+
+Definition rev {A} (l : list A) := itrev l [].
+
+Lemma lem_itrev {A} :
+  forall l acc : list A, itrev l acc = itrev l [] ++ acc.
+Proof.
+  induction l as [| h t IH].
+  - auto.
+  - intro acc.
+    simpl.
+    rewrite IH.
+    pattern (itrev t [h]).
+    rewrite IH.
+    rewrite <- List.app_assoc.
+    reflexivity.
+Qed.
+
+From Hammer Require Import Hints.
+(* The Hints module provides the following rewrite hint databases:
+   shints, slist, sbool, sarith, szarith. *)
+
+Lemma lem_itrev' {A} :
+  forall l acc : list A, itrev l acc = itrev l [] ++ acc.
+Proof.
+  (* induction l; sauto db: slist. *)
+  induction l; ssimpl.
+  (* Simplification tactics in the order of increasing strength and
+     decreasing speed: "simp_hyps", "sintuition", "qsimpl",
+     "ssimpl". *)
+  (* The simplification tactics may change the context in an
+     unpredictable manner and introduce automatically generated
+     hypothesis names. *)
+  rewrite IHl.
+  (* rewrite IHl. *)
+  pattern (itrev l [a]).
+  rewrite IHl.
+  sauto db: slist. (* The "slist" database contains "List.app_assoc" *)
+  (* "sauto" is currently not very good at rewriting - it just tries
+     to apply the "rewrite" tactic *)
+
+  Restart.
+
+  induction l as [|x l ?]; simpl.
+  - sauto.
+  - assert (itrev l [x] = itrev l [] ++ [x]) by sauto.
+    sauto db: slist.
+Qed.
+
+Lemma lem_rev_app {A} :
+  forall l1 l2 : list A, rev (l1 ++ l2) = rev l2 ++ rev l1.
+Proof.
+  unfold rev.
+  induction l1 as [| x l1 IH]; intro l2.
+  - simpl.
+    rewrite List.app_nil_r.
+    reflexivity.
+  - simpl.
+    rewrite lem_itrev.
+    rewrite IH.
+    rewrite <- List.app_assoc.
+    rewrite (lem_itrev l1 [x]).
+    reflexivity.
+Qed.
+
+Lemma lem_rev_app' {A} :
+  forall l1 l2 : list A, rev (l1 ++ l2) = rev l2 ++ rev l1.
+Proof.
+  unfold rev.
+  induction l1; sauto use: @lem_itrev db: slist.
+Qed.
+
+Lemma lem_rev_rev {A} : forall l : list A, rev (rev l) = l.
+Proof.
+  unfold rev.
+  induction l as [| x l IH].
+  - reflexivity.
+  - simpl.
+    rewrite (lem_itrev l [x]).
+    generalize (lem_rev_app (itrev l []) [x]).
+    unfold rev.
+    intro H.
+    rewrite H.
+    clear H.
+    rewrite IH.
+    reflexivity.
+Qed.
+
+Lemma lem_rev_rev' {A} : forall l : list A, rev (rev l) = l.
+Proof.
+  unfold rev.
+  (* induction l; sauto use: @lem_itrev, @lem_rev_app unfold: rev. *)
+  (* induction l; sauto limit: 2000 use: @lem_itrev, @lem_rev_app unfold: rev. *)
+  induction l as [|x l ?].
+  - reflexivity.
+  - sauto use: (lem_itrev l [x]), (lem_rev_app (itrev l []) [x]).
+Qed.
+
+Lemma lem_rev_lst {A} : forall l : list A, rev l = List.rev l.
+Proof.
+  unfold rev.
+  induction l as [|x l IH].
+  - reflexivity.
+  - simpl.
+    rewrite lem_itrev.
+    rewrite IH.
+    reflexivity.
+Qed.
+
+Lemma lem_rev_lst' {A} : forall l : list A, rev l = List.rev l.
+Proof.
+  unfold rev.
+  induction l; sauto use: @lem_itrev.
+Qed.
+
+Require Import Sorting.Permutation.
+
+Lemma lem_itrev_perm {A} :
+  forall l l' : list A, Permutation (itrev l l') (l ++ l').
+Proof.
+  induction l as [| x l IH]; simpl.
+  - eauto using Permutation.
+  - intro l'.
+    enough (Permutation (l ++ (x :: l')) (x :: l ++ l')).
+    { eauto using Permutation. }
+    eauto using Permutation_middle, Permutation_sym.
+Qed.
+
+Lemma lem_itrev_perm' {A} :
+  forall l l' : list A, Permutation (itrev l l') (l ++ l').
+Proof.
+  induction l; sauto use: Permutation_middle, Permutation_sym.
+Qed.
+
+Lemma lem_rev_perm {A} : forall l : list A, Permutation (rev l) l.
+Proof.
+  unfold rev.
+  intro l.
+  rewrite List.app_nil_end.
+  apply lem_itrev_perm.
+Qed.
+
+Lemma lem_rev_perm' {A} : forall l : list A, Permutation (rev l) l.
+Proof.
+  sauto use: @lem_itrev_perm db: slist unfold: rev.
+Qed.
